@prefix dc: <http://purl.org/dc/elements/1.1/> .
@prefix ov: <http://open.vocab.org/terms/> .
@prefix edm: <http://www.europeana.eu/schemas/edm/> .
@prefix foaf: <http://xmlns.com/foaf/0.1/> .
@prefix lingvo: <http://www.lingvoj.org/ontology#> .
@prefix void: <http://rdfs.org/ns/void#> .
@prefix ore: <http://www.openarchives.org/ore/terms/> .
@prefix dm2e-onto: <http://onto.dm2e.eu/schemas/dm2e/> .
@prefix dcterms: <http://purl.org/dc/terms/> .
@prefix rdfs: <http://www.w3.org/2000/01/rdf-schema#> .
@prefix bibo: <http://purl.org/ontology/bibo/> .
@prefix pro: <http://purl.org/spar/pro/> .
@prefix owl: <http://www.w3.org/2002/07/owl#> .
@prefix rdf: <http://www.w3.org/1999/02/22-rdf-syntax-ns#> .
@prefix dm2edata: <http://data.dm2e.eu/data/> .
@prefix skos: <http://www.w3.org/2008/05/skos#> .
@prefix csm: <http://www.mozajka.co/LOD/MM/> .

## New Concepts pertaining for the description of Codex Suprasliensis

csm:Fragment a skos:Concept ;
      rdfs:comment  "Physical part of a medieval manuscript."@en  ;
	  rdfs:label  "fragment"@en .
	  
csm:Line a skos:Concept ;
      rdfs:comment "A line of a written text."@en   ;
	  rdfs:label  "line"@en .

## New object properties for the description of Codex Suprasliensis

csm:startsAtLine a owl:ObjectProperty ;
     rdfs:comment "This property shows the line of the beginning of a work in a medieval manuscript."@en ;
	 rdfs:label "starts at line"@en ;
     rdfs:domain dm2e-onto:Work ;
     rdfs:range dm2e-onto:Page .

csm:endsAtLine a owl:ObjectProperty ;
     rdfs:comment "This property shows the line of the end of a work in a medieval manuscript."@en ;
	 rdfs:label "ends at line"@en ;
     rdfs:domain dm2e-onto:Work ;
     rdfs:range dm2e-onto:Page .

csm:readingFor a owl:ObjectProperty ;
	rdfs:comment "This property links a medieval work from a manuscript to the day from the church calendar in which the work is read during the church service."@en
	rdfs:label reading for"@en ;
	rdfs:domain dm2e-onto:Work ;
	rdfs:ranewge edm:TimeSpan .

## New datatype properties for the description of Codex Suprasliensis

csm:script a owl:DatatypeProperty ;
     rdfs:comment "This property indicates style of the script of a folio from a medieval manuscript."@en  ;
	 rdfs:label "script"@en ;
     rdfs:domain dm2e-onto:Page ;
	 rdfs:subPropertyOf dc:description .
	 
csm:inkColour a owl:DatatypeProperty ;
     rdfs:comment "This property indicates colour of the ink on a folio from a medieval manuscript."@en  ;
	 rdfs:label "ink colour"@en ;
     rdfs:domain dm2e-onto:Page ;
	 rdfs:subPropertyOf dc:description .





